pulse/pulse2rust/src/Pulse2Rust.Rust.Syntax.fst
@@ -62,10 +62,10 @@ let mk_option_typ (t:typ) : typ =
 let mk_array_typ (t:typ) (len:expr) : typ =
   Typ_array { typ_array_elem = t; typ_array_len = len }
 
-let mk_named_typ (s:string) (generic_args:list typ) : typ =
-  Typ_path [
-    { typ_path_segment_name = s; typ_path_segment_generic_args = generic_args };
-  ]
+let mk_named_typ (path:list typ_path_segment) (s:string) (generic_args:list typ) : typ =
+  Typ_path
+    (List.append path
+       [ { typ_path_segment_name = s; typ_path_segment_generic_args = generic_args } ])
 
 let mk_fn_typ (typ_fn_args:list typ) (typ_fn_ret:typ) : typ =
   Typ_fn { typ_fn_args; typ_fn_ret }
